EvaluationContexts.v
@@ -1,0 +1,219 @@
+(** Formal Reasoning About Programs <http://adam.chlipala.net/frap/>
+  * Chapter 12: More on Evaluation Contexts
+  * Author: Adam Chlipala
+  * License: https://creativecommons.org/licenses/by-nc-nd/4.0/ *)
+
+Require Import Frap.
+
+
+Module Stlc.
+  Inductive exp : Set :=
+  | Var (x : var)
+  | Const (n : nat)
+  | Plus (e1 e2 : exp)
+  | Abs (x : var) (e1 : exp)
+  | App (e1 e2 : exp).
+
+  Inductive value : exp -> Prop :=
+  | VConst : forall n, value (Const n)
+  | VAbs : forall x e1, value (Abs x e1).
+
+  Fixpoint subst (e1 : exp) (x : string) (e2 : exp) : exp :=
+    match e2 with
+      | Var y => if y ==v x then e1 else Var y
+      | Const n => Const n
+      | Plus e2' e2'' => Plus (subst e1 x e2') (subst e1 x e2'')
+      | Abs y e2' => Abs y (if y ==v x then e2' else subst e1 x e2')
+      | App e2' e2'' => App (subst e1 x e2') (subst e1 x e2'')
+    end.
+
+  Inductive context : Set :=
+  | Hole : context
+  | Plus1 : context -> exp -> context
+  | Plus2 : exp -> context -> context
+  | App1 : context -> exp -> context
+  | App2 : exp -> context -> context.
+
+  Inductive plug : context -> exp -> exp -> Prop :=
+  | PlugHole : forall e, plug Hole e e
+  | PlugPlus1 : forall e e' C e2,
+    plug C e e'
+    -> plug (Plus1 C e2) e (Plus e' e2)
+  | PlugPlus2 : forall e e' v1 C,
+    value v1
+    -> plug C e e'
+    -> plug (Plus2 v1 C) e (Plus v1 e')
+  | PlugApp1 : forall e e' C e2,
+    plug C e e'
+    -> plug (App1 C e2) e (App e' e2)
+  | PlugApp2 : forall e e' v1 C,
+    value v1
+    -> plug C e e'
+    -> plug (App2 v1 C) e (App v1 e').
+
+  (* Small-step, call-by-value evaluation, using our evaluation contexts *)
+
+  (* First: the primitive reductions *)
+  Inductive step0 : exp -> exp -> Prop :=
+  | Beta : forall x e v,
+    value v
+    -> step0 (App (Abs x e) v) (subst v x e)
+  | Add : forall n1 n2,
+    step0 (Plus (Const n1) (Const n2)) (Const (n1 + n2)).
+
+  (* Then: running them in context *)
+  Inductive step : exp -> exp -> Prop :=
+  | StepRule : forall C e1 e2 e1' e2',
+    plug C e1 e1'
+    -> plug C e2 e2'
+    -> step0 e1 e2
+    -> step e1' e2'.
+
+  (* It's easy to wrap everything as a transition system. *)
+  Definition trsys_of (e : exp) := {|
+    Initial := {e};
+    Step := step
+  |}.
+
+
+  (* Typing details are the same as last chapter. *)
+  Inductive type :=
+  | Nat                  (* Numbers *)
+  | Fun (dom ran : type) (* Functions *).
+
+  Inductive hasty : fmap var type -> exp -> type -> Prop :=
+  | HtVar : forall G x t,
+    G $? x = Some t
+    -> hasty G (Var x) t
+  | HtConst : forall G n,
+    hasty G (Const n) Nat
+  | HtPlus : forall G e1 e2,
+    hasty G e1 Nat
+    -> hasty G e2 Nat
+    -> hasty G (Plus e1 e2) Nat
+  | HtAbs : forall G x e1 t1 t2,
+    hasty (G $+ (x, t1)) e1 t2
+    -> hasty G (Abs x e1) (Fun t1 t2)
+  | HtApp : forall G e1 e2 t1 t2,
+    hasty G e1 (Fun t1 t2)
+    -> hasty G e2 t1
+    -> hasty G (App e1 e2) t2.
+
+  Local Hint Constructors value plug step0 step hasty : core.
+
+  Infix "-->" := Fun (at level 60, right associativity).
+  Coercion Const : nat >-> exp.
+  Infix "^+^" := Plus (at level 50).
+  Coercion Var : var >-> exp.
+  Notation "\ x , e" := (Abs x e) (at level 51).
+  Infix "@" := App (at level 49, left associativity).
+
+  (** * Now we adapt the automated proof of type soundness. *)
+
+  Ltac t0 := match goal with
+             | [ H : ex _ |- _ ] => invert H
+             | [ H : _ /\ _ |- _ ] => invert H
+             | [ |- context[?x ==v ?y] ] => cases (x ==v y)
+             | [ H : Some _ = Some _ |- _ ] => invert H
+
+             | [ H : step _ _ |- _ ] => invert H
+             | [ H : step0 _ _ |- _ ] => invert1 H
+             | [ H : hasty _ ?e _, H' : value ?e |- _ ] => invert H'; invert H
+             | [ H : hasty _ _ _ |- _ ] => invert1 H
+             | [ H : plug _ _ _ |- _ ] => invert1 H
+             end; subst.
+
+  Ltac t := simplify; propositional; repeat (t0; simplify); try equality; eauto 6.
+
+  Lemma progress : forall e t,
+    hasty $0 e t
+    -> value e
+    \/ (exists e' : exp, step e e').
+  Proof.
+    induct 1; t.
+  Qed.
+
+  Lemma weakening_override : forall (G G' : fmap var type) x t,
+    (forall x' t', G $? x' = Some t' -> G' $? x' = Some t')
+    -> (forall x' t', G $+ (x, t) $? x' = Some t'
+                      -> G' $+ (x, t) $? x' = Some t').
+  Proof.
+    simplify.
+    cases (x ==v x'); simplify; eauto.
+  Qed.
+
+  Local Hint Resolve weakening_override : core.
+
+  Lemma weakening : forall G e t,
+    hasty G e t
+    -> forall G', (forall x t, G $? x = Some t -> G' $? x = Some t)
+      -> hasty G' e t.
+  Proof.
+    induct 1; t.
+  Qed.
+
+  Local Hint Resolve weakening : core.
+
+  (* Replacing a typing context with an equal one has no effect (useful to guide
+   * proof search as a hint). *)
+  Lemma hasty_change : forall G e t,
+    hasty G e t
+    -> forall G', G' = G
+      -> hasty G' e t.
+  Proof.
+    t.
+  Qed.
+
+  Local Hint Resolve hasty_change : core.
+
+  Lemma substitution : forall G x t' e t e',
+    hasty (G $+ (x, t')) e t
+    -> hasty $0 e' t'
+    -> hasty G (subst e' x e) t.
+  Proof.
+    induct 1; t.
+  Qed.
+
+  Local Hint Resolve substitution : core.
+
+  Lemma preservation0 : forall e1 e2,
+    step0 e1 e2
+    -> forall t, hasty $0 e1 t
+      -> hasty $0 e2 t.
+  Proof.
+    invert 1; t.
+  Qed.
+
+  Local Hint Resolve preservation0 : core.
+
+  Lemma generalize_plug : forall e1 C e1',
+    plug C e1 e1'
+    -> forall e2 e2', plug C e2 e2'
+      -> (forall t, hasty $0 e1 t -> hasty $0 e2 t)
+      -> (forall t, hasty $0 e1' t -> hasty $0 e2' t).
+  Proof.
+    induct 1; t.
+  Qed.
+
+  Local Hint Resolve generalize_plug : core.
+
+  Lemma preservation : forall e1 e2,
+    step e1 e2
+    -> forall t, hasty $0 e1 t
+      -> hasty $0 e2 t.
+  Proof.
+    invert 1; t.
+  Qed.
+
+  Local Hint Resolve progress preservation : core.
+
+  Theorem safety : forall e t, hasty $0 e t
+    -> invariantFor (trsys_of e)
+                    (fun e' => value e'
+                               \/ exists e'', step e' e'').
+  Proof.
+    simplify.
+    apply invariant_weaken with (invariant1 := fun e' => hasty $0 e' t); eauto.
+    apply invariant_induction; simplify; eauto; equality.
+  Qed.
+End Stlc.
